high2/Zeta.High.Interleave.fsti
@@ -158,18 +158,6 @@ val eac_state_active_implies_prev_add (#app #n:_) (k: base_key) (il: eac_log app
 val eac_state_init_implies_no_key_refs (#app #n:_) (k: base_key) (il: eac_log app n)
   : Lemma (ensures (eac_state_of_key k il = EACInit ==> ~ (has_some_ref_to_key k il)))
 
-(* when the eac_state of k is instore, then k is in the store of a unique verifier thread *)
-val stored_tid (#app:_) (#n:nat) (k: base_key) (il: eac_log app n {EACInStore? (eac_state_of_key k il)})
-  : tid:nat{tid < n /\ store_contains (thread_store tid il) k}
-
-val lemma_instore (#app #n:_) (bk: base_key{bk <> Zeta.BinTree.Root}) (il: eac_log app n)
-  : Lemma (ensures (exists_in_some_store bk il <==> EACInStore? (eac_state_of_key bk il)))
-
-(* uniqueness: k is never in two stores *)
-val key_in_unique_store (#app #n:_) (k:base_key) (il: eac_log app n) (tid1 tid2: thread_id il)
-  : Lemma (ensures (tid1 <> tid2 ==>
-                    ~ (store_contains (thread_store tid1 il) k /\ store_contains (thread_store tid2 il) k)))
-
 let to_gen_key (#app #n:_) (bk: base_key) (il: eac_log app n {is_eac_state_active bk il \/ is_merkle_key bk})
   : gk:key app {to_base_key gk = bk}
   = if is_merkle_key bk then IntK bk
@@ -180,10 +168,20 @@ let to_gen_key (#app #n:_) (bk: base_key) (il: eac_log app n {is_eac_state_activ
       | EACEvictedBlum gk _ _ _ -> gk
       | EACEvictedMerkle gk _ -> gk
 
-val stored_key_is_correct (#app #n:_) (bk: base_key) (il: eac_log app n{EACInStore? (eac_state_of_key bk il)})
-  : Lemma (ensures (let tid = stored_tid bk il in
-                    let st = thread_store tid il in
-                    stored_key st bk = to_gen_key bk il))
+(* when the eac_state of k is instore, then k is in the store of a unique verifier thread *)
+val stored_tid (#app:_) (#n:nat) (k: base_key) (il: eac_log app n {EACInStore? (eac_state_of_key k il)})
+  : tid:nat{tid < n /\
+          (let st = thread_store tid il in
+           let gk = to_gen_key k il in
+           store_contains st k /\ gk = stored_key st k)}
+
+val lemma_instore (#app #n:_) (bk: base_key{bk <> Zeta.BinTree.Root}) (il: eac_log app n)
+  : Lemma (ensures (exists_in_some_store bk il <==> EACInStore? (eac_state_of_key bk il)))
+
+(* uniqueness: k is never in two stores *)
+val key_in_unique_store (#app #n:_) (k:base_key) (il: eac_log app n) (tid1 tid2: thread_id il)
+  : Lemma (ensures (tid1 <> tid2 ==>
+                    ~ (store_contains (thread_store tid1 il) k /\ store_contains (thread_store tid2 il) k)))
 
 let stored_value (#app #n:_) (gk: key app) (il: eac_log app n{EACInStore? (eac_state_of_gkey gk il)})
   : value_t gk
@@ -214,8 +212,11 @@ val eac_value_is_stored_value (#app #n:_) (il: eac_log app n) (gk: key app) (tid
                      store_contains (thread_store tid il) bk /\
                      stored_key (thread_store tid il) bk = gk))
           (ensures (let bk = to_base_key gk in
-                    EACInStore? (eac_state_of_key bk il) /\
                     eac_value gk il = HV.stored_value (thread_store tid il) bk))
+
+val eac_value_is_stored_value_int (#app #n:_) (il: eac_log app n) (k: merkle_key) (tid: nat{ tid < n })
+  : Lemma (requires (store_contains (thread_store tid il) k))
+          (ensures (eac_value (IntK k) il = HV.stored_value (thread_store tid il) k))
 
 let eac_state_evicted_value (#app #bk:_) (es: eac_state app bk {EAC.is_eac_state_evicted es})
   : value app
@@ -230,6 +231,13 @@ val eac_value_is_evicted_value (#app #n:_) (il: eac_log app n) (gk: key app):
         (ensures (let bk = to_base_key gk in
                   let es = eac_state_of_key bk il in
                   eac_state_evicted_value es = eac_value gk il))
+
+val eac_value_init_state_is_init (#app #n:_) (il: eac_log app n) (gk: key app):
+  Lemma (requires (let bk = to_base_key gk in
+                   let es = eac_state_of_key bk il in
+                   bk <> Zeta.BinTree.Root /\
+                   (es = EACInit \/ to_gen_key bk il <> gk)))
+        (ensures (eac_value gk il = init_value gk))
 
 val eac_value_init
   (#app #n:_)
